language_formal/spark2014_semantics/nested_array_record/monad.v
@@ -1,0 +1,116 @@
+
+
+Notation "'Let' 'some' x ':=' t 'in' u " :=
+  (match t with
+       Some x => u
+     | None => None
+   end)
+    (at level 60,right associativity,
+    format "'[' 'Let'  'some'  x  ':=' '/ ' '['  t  ']' 'in'  '//' u ']'")
+  : option_monad_scope.
+
+Notation "'Let' 'someb' x ':=' t 'in' u " :=
+  (match t with
+       Some x => u
+     | None => false
+   end)
+    (at level 60,right associativity,
+    format "'[' 'Let'  'someb'  x  ':=' '/ ' '['  t  ']' 'in'  '//' u ']'")
+  : option_monad_scope.
+
+Notation Return := Some (only parsing).
+
+Module EXAMPLE.
+  Open Scope option_monad_scope.
+  Definition essai1 := Return 1.
+
+  Definition essai :=
+    Let some x := Return 1 in
+    Let some y := Return 2 in
+    Return (x+y)%nat.
+
+  Eval compute in essai.
+
+End EXAMPLE.
+
+(*
+Inductive Result (TypeExc A:Type) : Type :=
+  Return: A -> Result TypeExc A
+| Raise: TypeExc -> Result TypeExc A.
+
+Arguments Raise {TypeExc} {A} _.
+Arguments Return {TypeExc} {A} _.
+
+(* Definition Return {A:Type} : A -> (A + E) := @inl A E. *)
+
+
+Definition Bind {TypeExc A B:Type} (x:Result TypeExc A) (f:A -> Result TypeExc B): Result TypeExc B :=
+  match x with
+    | Return x => (f x)
+    | Raise e => Raise e
+  end.
+
+Definition TryLet {TypeExc TypeExc' A B:Type} (x:Result TypeExc A) (f:A -> Result TypeExc' B)
+           (catch:TypeExc -> Result TypeExc' B): Result TypeExc' B :=
+  match x with
+    | Return x => f x
+    | Raise e => catch e
+  end.
+
+
+
+Notation "'Let' 'val' x ':=' t 'in' u " :=
+  (match t with
+       Return x => u
+     | Raise e => Raise e
+   end)
+    (at level 60,right associativity,
+    format "'[' 'Let'  'val'  x  ':=' '/ ' '['  t  ']' 'in'  '//'  u ']'").
+
+Notation "'try' t 'with' e '=>' u " :=
+  (match t with
+       Return x => Return x
+     | Raise e => u
+   end)
+    (at level 60,only parsing).
+
+
+Notation "'Lettry' 'val' t ':=' v 'in' f 'catch' e => catche " :=
+  (match v with
+    | Return t => f
+    | Raise e => catche
+  end)
+    (at level 60,only parsing).
+
+
+
+Definition BindO {A B:Type} (x:option A) (f:A -> option B): option B :=
+  match x with
+    | Some x => f x
+    | None => None
+  end.
+
+Notation "'Let' 'some' x ':=' t 'in' u " :=
+  (match t with Some x => u | None => None end)
+    (at level 60,right associativity,
+    format "'[' 'Let'  'some'  x  ':=' '/ ' '['  t  ']' 'in'  '//'  u ']'").
+
+
+
+Definition essai1 := @Return unit _ 1.
+(*
+Definition essai :=
+  Let val x := Return 1 in
+  Let val y := Return 2 in
+  Return (x+y)%nat.
+
+Definition essai3 :=
+  try
+    Let val x := Return 1 in
+    Let val y := Raise tt in
+    Return (x+y)%nat
+  with e => (Return 42).
+
+Eval compute in essai3.
+*)
+*)
