language_formal/spark2014_semantics/nested_array_record/semantics.v
@@ -1,0 +1,2221 @@
+Require Import util.
+Require Import LibTactics.
+Require Import more_list.
+Require Export values.
+Require Export environment.
+Require Export checks.
+
+Module Entry_val <: Entry.
+
+  Definition T := val.
+
+End Entry_val.
+
+Module STACK := ENV(Entry_val).
+Import STACK.
+
+(** * Relational Semantics (big-step) *)
+(** interpret the literal expressions *)
+Definition eval_literal (l: literal): value :=
+    match l with
+    | Integer_Literal v => BasicV (Int v)
+    | Boolean_Literal b => BasicV (Bool b)
+    end.
+
+(** interpret the binary operators *)
+Inductive eval_bin_expr: binary_operator -> value -> value -> value -> Prop :=
+    | Bin_Eq: forall v1 v2 b,
+        Zeq_bool v1 v2 = b ->
+        eval_bin_expr Equal (BasicV (Int v1)) (BasicV (Int v2)) (BasicV (Bool b))
+    | Bin_Ne: forall v1 v2 b,
+        Zneq_bool v1 v2 = b ->
+         eval_bin_expr Not_Equal (BasicV (Int v1)) (BasicV (Int v2)) (BasicV (Bool b))
+    | Bin_Gt: forall v1 v2 b,
+        Zgt_bool v1 v2 = b ->
+        eval_bin_expr Greater_Than (BasicV (Int v1)) (BasicV (Int v2)) (BasicV (Bool b))
+    | Bin_Ge: forall v1 v2 b,
+        Zge_bool v1 v2 = b ->
+        eval_bin_expr Greater_Than_Or_Equal (BasicV (Int v1)) (BasicV (Int v2)) (BasicV (Bool b))
+    | Bin_Lt: forall v1 v2 b,
+        Zlt_bool v1 v2 = b ->
+        eval_bin_expr Less_Than (BasicV (Int v1)) (BasicV (Int v2)) (BasicV (Bool b))
+    | Bin_Le: forall v1 v2 b,
+        Zle_bool v1 v2 = b ->
+        eval_bin_expr Less_Than_Or_Equal (BasicV (Int v1)) (BasicV (Int v2)) (BasicV (Bool b))
+    | Bin_And: forall v1 v2 b,
+        andb v1 v2 = b ->
+        eval_bin_expr And (BasicV (Bool v1)) (BasicV (Bool v2)) (BasicV (Bool b))
+    | Bin_Or: forall v1 v2 b,
+        orb v1 v2 = b ->
+        eval_bin_expr Or (BasicV (Bool v1)) (BasicV (Bool v2)) (BasicV (Bool b))
+    | Bin_Plus: forall v1 v2 v3,
+        (v1 + v2)%Z =v3 ->
+        eval_bin_expr Plus (BasicV (Int v1)) (BasicV (Int v2)) (BasicV (Int v3))
+    | Bin_Minus: forall v1 v2 v3,
+        (v1 - v2)%Z =v3 ->
+        eval_bin_expr Minus (BasicV (Int v1)) (BasicV (Int v2)) (BasicV (Int v3))
+    | Bin_Mul: forall v1 v2 v3,
+        (v1 * v2)%Z =v3 ->
+        eval_bin_expr Multiply (BasicV (Int v1)) (BasicV (Int v2)) (BasicV (Int v3))
+    | Bin_Div: forall v1 v2 v3,
+        (Z.quot v1 v2)%Z =v3 ->
+        eval_bin_expr Divide (BasicV (Int v1)) (BasicV (Int v2)) (BasicV (Int v3)).
+
+(** interpret the unary operation *)
+Inductive eval_unary_expr : unary_operator -> value -> value -> Prop :=
+    | Unary_Not: forall b v,
+        negb b = v ->
+        eval_unary_expr Not (BasicV (Bool b)) (BasicV (Bool v))
+    | EUnary_Plus: forall v,
+        eval_unary_expr Unary_Plus (BasicV (Int v)) (BasicV (Int v)).
+
+Lemma eval_bin_unique: forall op v1 v2 x y,
+    eval_bin_expr op v1 v2 x ->
+    eval_bin_expr op v1 v2 y ->
+    x = y.
+Proof.
+    intros.
+    destruct op;
+    inversion H; subst; inversion H0; subst;
+    auto.
+Qed.
+
+Lemma eval_unary_unique: forall uop v x y,
+    eval_unary_expr uop v x ->
+    eval_unary_expr uop v y ->
+    x = y.
+Proof.
+    intros.
+    destruct uop;
+    inversion H; subst; inversion H0; subst;
+    auto.
+Qed.
+
+
+(** ** Expression semantics *)
+(**
+    for binary expression and unary expression, if a run time error 
+    is detected in any of its child expressions, then return a run
+    time error; for binary expression (e1 op e2), if both e1 and e2 
+    are evaluated to some normal value, then run time checks are
+    performed according to the checking rules specified for the 
+    operator 'op', whenever the check fails (returning false), a run 
+    time error is detected and the program is terminated, otherwise, 
+    normal binary operation result is returned;
+*)
+
+Inductive eval_expr: stack -> expression -> Return value -> Prop :=
+    | eval_E_Literal: forall l v s ast_num,
+        eval_literal l = v ->
+        eval_expr s (E_Literal ast_num l) (Normal v)
+    | eval_E_Identifier: forall x s v ast_num,
+        fetchG x s = Some (Value v) ->
+        eval_expr s (E_Identifier ast_num x) (Normal v)
+    | eval_E_Binary_Operation1: forall s e1 ast_num op e2,
+        eval_expr s e1 Run_Time_Error ->
+        eval_expr s (E_Binary_Operation ast_num op e1 e2) Run_Time_Error
+    | eval_E_Binary_Operation2: forall s e1 v1 e2 ast_num op,
+        eval_expr s e1 (Normal v1) ->
+        eval_expr s e2 Run_Time_Error ->
+        eval_expr s (E_Binary_Operation ast_num op e1 e2) Run_Time_Error
+    | eval_E_Binary_Operation3: forall s e1 v1 e2 v2 ast_num op,
+        eval_expr s e1 (Normal v1) ->
+        eval_expr s e2 (Normal v2) ->
+        do_check op v1 v2 false ->
+        eval_expr s (E_Binary_Operation ast_num op e1 e2) Run_Time_Error
+    | eval_E_Binary_Operation4: forall s e1 v1 e2 v2 ast_num op v,
+        eval_expr s e1 (Normal v1) ->
+        eval_expr s e2 (Normal v2) ->
+        do_check op v1 v2 true ->
+        eval_bin_expr op v1 v2 v ->
+        eval_expr s (E_Binary_Operation ast_num op e1 e2) (Normal v)
+    | eval_E_Unary_Operation1: forall s e ast_num op,
+        eval_expr s e Run_Time_Error ->
+        eval_expr s (E_Unary_Operation ast_num op e) Run_Time_Error
+    | eval_E_Unary_Operation2: forall s e v ast_num op v1,
+        eval_expr s e (Normal v) ->
+        eval_unary_expr op v v1 ->
+        eval_expr s (E_Unary_Operation ast_num op e) (Normal v1)
+    | eval_E_Aggregate: forall s a v ast_num,
+        eval_aggregate s a v ->
+        eval_expr s (E_Aggregate ast_num a) v
+    | eval_E_Name: forall s n v ast_num,
+        eval_name s n v -> 
+        eval_expr s (E_Name ast_num n) v
+
+with eval_aggregate : stack -> aggregate -> Return value -> Prop :=
+    | eval_Record_Aggregate: forall s lrca v ast_num,
+        eval_list_record_component_association s lrca v ->
+        eval_aggregate s (Record_Aggregate ast_num lrca) v
+    | eval_Array_Aggregate: forall s aa v ast_num,
+        eval_array_aggregate s aa v ->
+        eval_aggregate s (Array_Aggregate ast_num aa) v
+
+with eval_array_aggregate : stack -> array_aggregate -> Return value -> Prop :=
+    | eval_Positional_Array_Aggregate: forall s pa v ast_num,
+        eval_positional_array_aggregate s pa v ->
+        eval_array_aggregate s (Positional_Array_Aggregate ast_num pa) v
+ (* | eval_Named_Array_Aggregate *)
+
+with eval_list_record_component_association : stack -> list record_component_association -> Return value -> Prop :=
+    | eval_Named_Component_Associations1: forall s e ast_num x lnca,
+        eval_expr s e Run_Time_Error ->
+        eval_list_record_component_association s ((Named_Component_Association ast_num x e) :: lnca) Run_Time_Error
+    | eval_Named_Component_Associations2: forall s e v ast_num x,
+        eval_expr s e (Normal v) ->
+        eval_list_record_component_association s ((Named_Component_Association ast_num x e) :: nil) (Normal (AggregateV (RecordV ((x, v) :: nil))))
+    | eval_Named_Component_Associations3: forall s e v rca lrca ast_num x,
+        eval_expr s e (Normal v) ->
+        eval_list_record_component_association s (rca :: lrca) Run_Time_Error -> 
+        eval_list_record_component_association s ((Named_Component_Association ast_num x e) :: rca :: lrca) Run_Time_Error 
+    | eval_Named_Component_Associations4: forall s e v rca lrca lv ast_num x,
+        eval_expr s e (Normal v) ->
+        eval_list_record_component_association s (rca :: lrca) (Normal (AggregateV (RecordV lv))) ->
+        eval_list_record_component_association s ((Named_Component_Association ast_num x e) :: rca :: lrca) (Normal (AggregateV (RecordV ((x, v) :: lv))))
+
+(*
+with eval_record_component_association : stack -> record_component_association -> Return value -> Prop :=
+    | eval_Positional_Component_Association
+    | eval_Named_Component_Associatio
+*)
+
+with eval_positional_array_aggregate : stack -> positional_array_aggregate -> Return value -> Prop :=
+    | eval_Positional_Array_Component_Association1: forall s le v astnum,
+        eval_list_exprs s le v ->
+        eval_positional_array_aggregate s (Positional_Array_Component_Association astnum le) v
+(*  | eval_Positional_Array_Component_Association_Others: 
+        ...
+        eval_positional_array_aggregate s (Positional_Array_Component_Association_Others astnum le others) v *)
+
+with eval_list_exprs: stack -> list expression -> Return value -> Prop := 
+    | eval_List_Exps1: forall s e le,
+        eval_expr s e Run_Time_Error ->
+        eval_list_exprs s (e :: le) Run_Time_Error
+    | eval_List_Exps2: forall s e v,
+        eval_expr s e (Normal v) ->
+        eval_list_exprs s (e :: nil) (Normal (AggregateV (ArrayV (v :: nil))))
+    | eval_List_Exps3: forall s e1 v1 e2 le,
+        eval_expr s e1 (Normal v1) ->
+        eval_list_exprs s (e2 :: le) Run_Time_Error ->
+        eval_list_exprs s (e1 :: e2 :: le) Run_Time_Error
+    | eval_List_Exps4: forall s e1 v1 e2 le lv,
+        eval_expr s e1 (Normal v1) ->
+        eval_list_exprs s (e2 :: le) (Normal (AggregateV (ArrayV lv))) ->
+        eval_list_exprs s (e1 :: e2 :: le) (Normal (AggregateV (ArrayV (v1 :: lv))))
+
+(*
+with name: Type := (* 4.1 *)
+        | Indexed_Component: astnum -> name -> list expression -> name (* 4.1.1 *)
+        | Selected_Component: astnum -> name -> idnum -> name          (* 4.1.3 *)
+*)
+with eval_name: stack -> name -> Return value -> Prop :=
+    | eval_Indexed_Component1: forall s n ast_num le,
+        eval_name s n Run_Time_Error ->
+        eval_name s (Indexed_Component ast_num n le) Run_Time_Error
+    | eval_Indexed_Component2: forall s n v le ast_num,
+        eval_name s n (Normal v) ->
+        eval_list_exprs s le Run_Time_Error ->
+        eval_name s (Indexed_Component ast_num n le) Run_Time_Error
+    | eval_Indexed_Component3: forall s n mapv le lv result ast_num,
+        eval_name s n (Normal (AggregateV (ArrayV mapv))) ->
+        eval_list_exprs s le (Normal (AggregateV (ArrayV lv))) ->
+        array_index_result mapv lv result ->
+        eval_name s (Indexed_Component ast_num n le) result
+    | eval_Selected_Component: forall s n ast_num x,
+        eval_name s n Run_Time_Error -> 
+        eval_name s (Selected_Component ast_num n x) Run_Time_Error
+
+with array_index_result: list value -> list value -> Return value -> Prop :=
+     | Index1: 
+         array_index_result nil nil Run_Time_Error
+.
+
+Fixpoint array_index (a: list value) (i: list value): Return value :=
+  match a with
+  | nil => Run_Time_Error
+  | (a1 :: al) => 
+      match i with
+      | 
+.
+
+
+
+(** * Statement semantics *)
+
+(** ** Stack manipulation for procedure calls and return *)
+
+(** [Copy_out prefix lparams lexp s s'] means that s' is the result of
+    copying Out params of the currently finished procedure of prefix
+    into there output variables. More precisely:
+  - [prefix] is a portion of stack where only the parameters of the
+    procedure are stored;
+  - [lparams] is the static specification of the parameters of the
+    procedure;
+  - [lexp] is the list of original expressions given as parameter of
+    the procedure (this is where one can find in which variables "out"
+    parameters must be copied);
+  - [s] is the portion of the stack which needs to be updated and
+    returned by the procedure, more precisely: it contains the global
+    parameters + the local environment of the colling procedure;
+  - [s'] is the resulting state. *)
+Inductive Copy_out: store -> list parameter_specification
+                    -> list expression -> stack -> stack -> Prop :=
+  Copy_out_nil : forall prf σ, Copy_out prf nil nil σ σ
+| Copy_out_cons_out:
+    forall σ σ' σ'' id v prf prm lprm lexp idorig astnum,
+      prm.(parameter_mode) = Out
+      -> id = prm.(parameter_name)
+      -> fetch id prf = Some v
+      -> updateG σ idorig v = Some σ'
+      -> Copy_out prf lprm lexp σ' σ''
+      -> Copy_out prf (prm::lprm) ((E_Identifier astnum idorig) :: lexp) σ σ''
+| Copy_out_cons_in:
+    forall σ σ'  prf prm lprm lexp e,
+      prm.(parameter_mode) = In
+      -> Copy_out prf lprm lexp σ σ'
+      -> Copy_out prf (prm::lprm) (e :: lexp) σ σ'.
+
+(** [Copy_in s lparams lexp frame] means the frame is the portion of
+    stack to push on the stack to start evaluating the procedure
+    having [lparams] as parameters spcification. More precisely,
+    [frame] contains the value of the formal parameters described by
+    [lpamrams]. These values are computed from the list of arguments
+    [lexp]. Only "In" parameters are evaluated, "Out" parameters are
+    set to [Undefined]. *)
+Inductive Copy_in: stack -> list parameter_specification
+                   -> list expression -> Return store -> Prop :=
+  Copy_in_nil : forall σ, Copy_in σ nil nil (Normal nil) 
+| Copy_in_cons_out:
+    forall σ lparam lexp (frame:store) prm idv ast_num,
+      Copy_in σ lparam lexp (Normal frame)
+      -> prm.(parameter_mode) = Out
+      -> Copy_in σ (prm::lparam) (E_Identifier ast_num idv::lexp)
+                 (Normal ((prm.(parameter_name),Undefined)::frame))
+| Copy_in_cons_out_rte:
+    forall σ lparam lexp prm idv ast_num,
+      Copy_in σ lparam lexp Run_Time_Error
+      -> prm.(parameter_mode) = Out
+      -> Copy_in σ (prm::lparam) (E_Identifier ast_num idv::lexp) Run_Time_Error
+| Copy_in_cons_in_rte1:
+    forall σ lparam lexp prm e,
+      prm.(parameter_mode) = In
+      -> eval_expr σ e Run_Time_Error
+      -> Copy_in σ (prm::lparam) (e::lexp) Run_Time_Error
+| Copy_in_cons_in_rte2:
+    forall σ lparam lexp prm e v,
+      Copy_in σ lparam lexp Run_Time_Error
+      -> eval_expr σ e (Normal v)
+      -> prm.(parameter_mode) = In
+      -> Copy_in σ (prm::lparam) (e::lexp) Run_Time_Error
+| Copy_in_cons_in:
+    forall σ lparam lexp frame prm e v,
+      Copy_in σ lparam lexp (Normal frame)
+      -> prm.(parameter_mode) = In
+      -> eval_expr σ e (Normal v)
+      -> Copy_in σ (prm::lparam) (e::lexp)
+                 (Normal ((prm.(parameter_name),Value v)::frame)).
+
+
+(** *** Inductive semantic of declarations. [eval_decl s nil decl
+        rsto] means that rsto is the frame to be pushed on s after
+        evaluating decl, sto is used as an accumulator for building
+        the frame.
+ *)
+Inductive eval_decl: stack -> store -> declaration -> Return store -> Prop :=
+| eval_Decl_E:
+    forall e d s sto,
+      Some e = d.(initialization_expression) ->
+      eval_expr (sto::s) e Run_Time_Error ->
+      eval_decl s sto (D_Object_declaration d) Run_Time_Error
+| eval_Decl:
+    forall d x e v s sto,
+      x = d.(object_name) ->
+      Some e = d.(initialization_expression) ->
+      eval_expr (sto::s) e (Normal v) ->
+      eval_decl s sto (D_Object_declaration d) (Normal ((x, Value v) :: sto))
+| eval_UndefDecl:
+    forall d x s sto,
+      x = d.(object_name) ->
+      None = d.(initialization_expression) ->
+      eval_decl s sto (D_Object_declaration d) (Normal ((x, Undefined) :: sto))
+| eval_decl_Seq:
+    forall dcl1 dcl2 s s' s'' sto,
+      eval_decl s sto dcl1 (Normal s') ->
+      eval_decl s s' dcl2 (Normal s'') ->
+      eval_decl s sto (D_Sequence dcl1 dcl2) (Normal s'')
+| eval_decl_Seq_err1:
+    forall dcl1 dcl2 s sto,
+      eval_decl s sto dcl1 Run_Time_Error ->
+      eval_decl s sto (D_Sequence dcl1 dcl2) Run_Time_Error
+| eval_decl_Seq_err2:
+    forall dcl1 dcl2 s s' sto,
+      eval_decl s sto dcl1 (Normal s') ->
+      eval_decl s s' dcl2 Run_Time_Error ->
+      eval_decl s sto (D_Sequence dcl1 dcl2) Run_Time_Error
+| eval_decl_proc:
+    forall s pbody sto,
+      eval_decl s sto (D_Procedure_declaration pbody)
+                (Normal ((procedure_name pbody,Procedure pbody)::sto)).
+
+(** ** Inductive semantic of statement and declaration
+
+   in a statement evaluation, whenever a run time error is detected in
+   the evaluation of its sub-statements or sub-component, the
+   evaluation is terminated and return a run time error; otherwise,
+   evaluate the statement into a normal state.
+
+ *)
+
+
+Inductive eval_stmt: stack -> statement -> Return stack -> Prop := 
+    | eval_S_Assignment1: forall s e ast_num x,
+        eval_expr s e Run_Time_Error ->
+        eval_stmt s (S_Assignment ast_num x e) Run_Time_Error
+    | eval_S_Assignment2: forall s e v x s1 ast_num,
+        eval_expr s e (Normal v) ->
+        updateG s x (Value v) = Some s1 ->
+        eval_stmt s (S_Assignment ast_num x e) (Normal s1)
+    | eval_S_Sequence1: forall s c1 ast_num c2,
+        eval_stmt s c1 Run_Time_Error ->
+        eval_stmt s (S_Sequence ast_num c1 c2) Run_Time_Error
+    | eval_S_Sequence2: forall ast_num s s1 s2 c1 c2,
+        eval_stmt s c1 (Normal s1) ->
+        eval_stmt s1 c2 s2 ->
+        eval_stmt s (S_Sequence ast_num c1 c2) s2
+    | eval_S_If: forall s b ast_num c,
+        eval_expr s b Run_Time_Error ->
+        eval_stmt s (S_If ast_num b c) Run_Time_Error
+    | eval_S_If_True: forall s b c s1 ast_num,
+        eval_expr s b (Normal (Bool true)) ->
+        eval_stmt s c s1 ->
+        eval_stmt s (S_If ast_num b c) s1
+    | eval_S_If_False: forall s b ast_num c,
+        eval_expr s b (Normal (Bool false)) ->
+        eval_stmt s (S_If ast_num b c) (Normal s)
+    | eval_S_While_Loop: forall s b ast_num c,
+        eval_expr s b Run_Time_Error ->
+        eval_stmt s (S_While_Loop ast_num b c) Run_Time_Error
+    | eval_S_While_Loop_True1: forall s b c ast_num,
+        eval_expr s b (Normal (Bool true)) ->
+        eval_stmt s c Run_Time_Error ->
+        eval_stmt s (S_While_Loop ast_num b c) Run_Time_Error
+    | eval_S_While_Loop_True2: forall s b c s1 ast_num s2,
+        eval_expr s b (Normal (Bool true)) ->
+        eval_stmt s c (Normal s1) ->
+        eval_stmt s1 (S_While_Loop ast_num b c) s2 ->
+        eval_stmt s (S_While_Loop ast_num b c) s2
+    | eval_S_While_Loop_False: forall s b ast_num c,
+        eval_expr s b (Normal (Bool false)) ->
+        eval_stmt s (S_While_Loop ast_num b c) (Normal s)
+    | eval_S_Proc_rteargs:
+        forall pbname (pb:procedure_declaration) lexp s ast_num,
+          fetchG pbname s = Some (Procedure pb) ->
+          Copy_in s (procedure_parameter_profile pb) lexp Run_Time_Error ->
+          eval_stmt s (S_ProcCall ast_num pbname lexp) Run_Time_Error
+    | eval_S_Proc_rtedecl:
+        forall pbname (pb:procedure_declaration) lexp s_caller s_forget s ast_num prefix,
+          fetchG pbname s_caller = Some (Procedure pb) ->
+          Copy_in s_caller (procedure_parameter_profile pb) lexp (Normal prefix) ->
+          Cut_until s_caller pbname s_forget s -> (* s_caller = s_forget++s *)
+          eval_decl s prefix (procedure_declarative_part pb) Run_Time_Error ->
+          eval_stmt s_caller (S_ProcCall ast_num pbname lexp) Run_Time_Error
+    | eval_S_Proc_rtebody:
+        forall pbname (pb:procedure_declaration) lexp s_caller s_forget s ast_num s2 prefix,
+          fetchG pbname s_caller = Some (Procedure pb) ->
+          Copy_in s_caller (procedure_parameter_profile pb) lexp (Normal prefix) ->
+          Cut_until s_caller pbname s_forget s -> (* s_caller = s_forget++s *)
+          eval_decl s prefix (procedure_declarative_part pb) (Normal s2) ->
+          eval_stmt (s2::s) (procedure_statements pb) Run_Time_Error ->
+          eval_stmt s_caller (S_ProcCall ast_num pbname lexp) Run_Time_Error
+    | eval_S_Proc:
+        forall pbname (pb:procedure_declaration) lexp s_caller s_forget s ast_num
+               s2 s3 s' s'' slocal prefix prefix',
+          fetchG pbname s_caller = Some (Procedure pb) ->
+          Copy_in s_caller (procedure_parameter_profile pb) lexp (Normal prefix) ->
+          Cut_until s_caller pbname s_forget s -> (* s_caller = s_forget++s *)
+          eval_decl s prefix (procedure_declarative_part pb) (Normal s2) ->          
+          eval_stmt (s2::s) (procedure_statements pb) (Normal s3) ->
+          s3 = (slocal ++ prefix') :: s' -> (* extract parameters from local frame *)
+          List.length prefix = List.length prefix' ->
+          Copy_out prefix' (procedure_parameter_profile pb) lexp (s_forget++s') s'' ->
+          eval_stmt s_caller (S_ProcCall ast_num pbname lexp) (Normal s'')
+.
+
+
+(** ** examples *)
+
+Module ExampleProcedures.
+(* EXAMPLE 1, v102 is a variable in the scope.
+------------------------
+procedure P2 () is
+  V4 : TYPE5 := 34;
+begin
+  V102 := 56;
+end 
+-----------------------
+*)
+Definition proc1:procedure_declaration := (mkprocedure_declaration
+           1 101 nil nil
+             (D_Object_declaration
+                {|
+                  declaration_astnum := 3;
+                  object_name := 4;
+                  object_nominal_subtype :=  5;
+                  initialization_expression := Some (E_Literal 6 (Integer_Literal(34)))
+                |}
+             )
+             (S_Assignment 12 102 (E_Literal 8 (Integer_Literal(56))))).
+
+Definition s1:stack := ((101,Procedure proc1) :: (102, Value (Int(77))) :: nil)::nil.
+
+Definition s2:stack := ((101,Procedure proc1) :: (102, Value (Int(56)))  :: nil)::nil.
+
+
+Lemma essai: eval_stmt s1 (S_ProcCall 13 101 nil) (Normal s2).
+Proof.
+  eapply eval_S_Proc; try now (simpl; eauto).
+  - simpl.
+    instantiate (1 := nil).
+    constructor.
+  - constructor 1.
+    reflexivity.
+    
+  - econstructor 2.
+    + reflexivity.
+    + simpl.
+      reflexivity.
+    + constructor.
+      simpl.
+      reflexivity.
+  - simpl.
+    econstructor.
+    + econstructor.
+      simpl.
+      eauto.
+    + simpl.
+      rewrite app_nil_r.
+      reflexivity.
+  - simpl.
+    constructor 1.
+Qed.
+
+
+
+(* v102 is a variable in the scope.
+procedure P2 () is
+  V4 : TYPE5 := 34;
+  V5 : TYPE5 := 37;
+begin
+  V5 := V4 + V5;
+  V102 := V5*2;
+end 
+*)
+Definition proc2:procedure_declaration := (mkprocedure_declaration
+           1 101 nil nil
+             (D_Sequence
+                (D_Object_declaration
+                   {|
+                     declaration_astnum := 3;
+                     object_name := 4;
+                     object_nominal_subtype :=  5;
+                     initialization_expression := Some (E_Literal 6 (Integer_Literal(34)))
+                   |}
+                )
+                (D_Object_declaration
+                   {|
+                     declaration_astnum := 4;
+                     object_name := 5;
+                     object_nominal_subtype :=  5;
+                     initialization_expression := Some (E_Literal 6 (Integer_Literal(37)))
+                   |}
+                )
+             )
+             (S_Sequence 13
+                (S_Assignment 14 5
+                              (E_Binary_Operation 9 Plus
+                                                  (E_Identifier 10 5)
+                                                  (E_Identifier 10 4)))
+                (S_Assignment
+                   12
+                   102
+                   (E_Binary_Operation 9 Multiply
+                                       (E_Identifier 10 5)
+                                       (E_Literal 8 (Integer_Literal(2))))))).
+
+Definition sto3:store := (101,Procedure proc2) :: (102, Value (Int(77))) :: nil.
+
+Definition sto4:store := (101,Procedure proc2) :: (102, Value (Int(142)))  :: nil.
+
+
+
+Lemma essai2: eval_stmt (sto3::nil) (S_ProcCall 13 101 nil) (Normal (sto4::nil)).
+Proof.
+  eapply eval_S_Proc; try now (simpl; eauto).
+  - simpl.
+    constructor.
+  - constructor 1.
+    reflexivity.
+  - 
+(*     instantiate (1:= ((5, Value (Int 37))::(4, Value (Int 34))::s3)). *)
+    unfold sto3, sto4, proc1.
+    simpl.
+    econstructor 4;simpl.
+    + econstructor 2;simpl.
+      * econstructor;eauto.
+      * reflexivity.
+      * constructor.
+        simpl.
+        reflexivity.
+    + econstructor 2;simpl.
+      * econstructor;eauto.
+      * reflexivity.
+      * constructor.
+        simpl.
+        reflexivity.
+  - simpl.
+    + { econstructor.
+        - econstructor.
+          + econstructor.
+            * econstructor.
+              simpl.
+              eauto.
+            * constructor.
+              simpl.
+              eauto.
+            * constructor.
+              vm_compute.
+              reflexivity.
+            * econstructor.
+              simpl.
+              eauto.
+          + simpl.
+            reflexivity.
+        - econstructor.
+          + econstructor.
+            * econstructor.
+              simpl.
+              eauto.
+            * econstructor.
+              simpl.
+              eauto.
+            * econstructor.
+              vm_compute.
+              reflexivity.
+            * econstructor.
+            simpl.
+            eauto.
+        + simpl.
+          rewrite app_nil_r.
+          reflexivity. }
+  - simpl.
+    constructor 1.
+Qed.
+
+
+End ExampleProcedures.
+(* END EXAMPLE *)  
+
+(** ** Functional Semantics of expressions *)
+
+(** for relational semantics of expression and statement, we also 
+    provide its corresponding version of functional semantics, and 
+    prove that they are semantics equivalent;
+    relational semantics encode the formal semantics rules, while
+    functional semantics is useful to familiarize oneself with the 
+    SPARK 2014 semantics, and validate it experimentally by testing, 
+    and it also helps to fix the program if the program exhibits 
+    undefined behavior;
+    
+    Bisimulation between relational and functional semantics are
+    proved for the following pairs of evaluations: 
+    
+    - f_eval_binexpr <-> eval_binexpr;
+    
+    - f_eval_unaryexpr <-> eval_unaryexpr;
+    
+    - f_eval_expr <-> eval_expr;
+
+    - f_eval_stmt <-> eval_stmt;
+*)
+
+(** *** semantic of operators *)
+
+(** interpret the binary operation for each binary operator *)
+Definition f_eval_bin_expr (op: binary_operator) (v1: value) (v2: value): Return value :=
+    match op with
+    | Equal => Val.eq v1 v2
+    | Not_Equal => Val.ne v1 v2
+    | Greater_Than => Val.gt v1 v2
+    | Greater_Than_Or_Equal => Val.ge v1 v2
+    | Less_Than => Val.lt v1 v2
+    | Less_Than_Or_Equal => Val.le v1 v2
+    | And => Val.and v1 v2
+    | Or => Val.or v1 v2
+    | Plus => Val.add v1 v2
+    | Minus => Val.sub v1 v2
+    | Multiply => Val.mul v1 v2
+    | Divide => Val.div v1 v2
+    end.
+
+(** interpret the unary operation *)
+Definition f_eval_unary_expr (op: unary_operator) (v: value): Return value :=
+    match op with
+    | Not => Val.not v
+    | Unary_Plus => Val.unary_add v
+    end.
+
+(** *** Expression semantics *)
+
+(** in functional semantics for expression, it returns either a
+    normal value or a run time error or go abnormal, the run time 
+    checks (for example, division by zero check) are encoded inside 
+    the semantics; *)
+Function f_eval_expr (s: stack) (e: expression): Return value :=
+    match e with
+    | E_Literal _ v => Normal (eval_literal v)
+    | E_Identifier _ x =>
+        match (fetchG x s) with
+        | Some (Value v) => Normal v
+        | _ => Abnormal (* None or not a value *)
+        end
+    | E_Binary_Operation _ op e1 e2 =>
+        match f_eval_expr s e1 with
+        | Normal v1 => 
+            match f_eval_expr s e2 with
+            | Normal v2 => 
+                match f_do_check op v1 v2 with
+                | Some true => f_eval_bin_expr op v1 v2
+                | Some false => Run_Time_Error
+                | _ => Abnormal
+                end
+            | Run_Time_Error => Run_Time_Error
+            | Abnormal => Abnormal
+            | Unterminated => Unterminated
+            end
+        | Run_Time_Error => Run_Time_Error
+        | Abnormal => Abnormal
+        | Unterminated => Unterminated
+        end   
+    | E_Unary_Operation _ op e => 
+        match f_eval_expr s e with
+        | Normal v => f_eval_unary_expr op v
+        | Run_Time_Error => Run_Time_Error
+        | Abnormal => Abnormal
+        | Unterminated => Unterminated
+        end
+    end.
+
+(** ** Functional Statement semantics *)
+
+
+(** *** Functional manipulation of the stack for procedure call and
+    retrun *)
+
+(** functional version of Copy_out
+  [copy_out prefx params lexp s'] returns s' updated in the following
+  way: for each param in params that is Out, pick the correponding
+  variable name in lexp and update s' with the value of the param that
+  is stored in prefix. *)
+Function copy_out (prefx:store) (params: list parameter_specification)
+         (lexp:list expression) (s: stack) {struct params}:  Return stack :=
+  match params, lexp with
+    | nil , nil => Normal s
+    | (prm::params') , (e::lexp') =>
+      match prm.(parameter_mode) with
+         | Out =>
+           match e with
+             | E_Identifier _ x =>
+               match (fetch (prm.(parameter_name)) prefx) with
+                   Some v =>
+                   match updateG s x v with
+                     | Some s' => copy_out prefx params' lexp' s'
+                     | None => Abnormal
+                   end
+                 | None => Abnormal
+               end
+             | _ => Abnormal
+           end
+         | In => copy_out prefx params' lexp' s
+         | _ => Abnormal
+       end
+    | _ , _ => Abnormal
+  end.
+
+(** Functional version of Copy_in.
+   [copy_in s lparams lexp] returns the prefix to push on the stack
+   before evaluationg procedure body (i.e. declaration block +
+   statement). "Out" parameters values are copied into there output
+   variables (stored in lexp). *)
+Function copy_in (s:stack) lparams lexp: Return store :=
+  match lparams,lexp with
+  | (prm :: lparams') , (exp:: lexp') =>
+    match prm.(parameter_mode) with
+      | Out => if is_var exp
+               then match copy_in s lparams' lexp' with
+                      | Normal res => Normal ((prm.(parameter_name), Undefined) :: res)
+                      | res => res
+                    end
+               else Abnormal
+      | In =>
+        let v := f_eval_expr s exp in
+        match v with
+          | Normal v' =>
+            match copy_in s lparams' lexp' with
+              | Normal res => Normal ((prm.(parameter_name), Value v') :: res)
+              | res => res
+            end
+          | Run_Time_Error => Run_Time_Error
+          | Abnormal => Abnormal
+          | Unterminated => Unterminated
+        end
+      | In_Out => Abnormal (* not yet implemented *)
+    end
+  | nil , nil => Normal nil
+  | _ , _ => Abnormal
+  end.
+
+(** *** functional semantic of declarations *)
+
+Function f_eval_decl (s: stack) (sto:store) (c: declaration) {struct c}: Return store :=
+  match c with
+    | D_Object_declaration d =>
+      match d.(initialization_expression) with
+        | Some e =>
+          match f_eval_expr (sto::s) e with
+            | Run_Time_Error => Run_Time_Error
+            | Normal v =>
+              (Normal ((d.(object_name), Value v)::sto))
+            | Abnormal => Abnormal
+            | Unterminated => Unterminated
+          end
+        | None => (Normal ((d.(object_name), Undefined) :: sto))
+      end
+    | D_Sequence dcl1 dcl2 =>
+      match f_eval_decl s sto dcl1 with
+        | Normal s' => f_eval_decl s s' dcl2
+        | err => err
+      end
+    | D_Procedure_declaration pbody =>
+      Normal((procedure_name pbody,Procedure pbody)::sto)
+  end.
+
+(** *** functional semantic of statements *)
+
+(** 
+   in the functional semantics for statement, 'k' denotes the execution 
+   steps, whenever it reaches 0, an untermination state is returned;
+   otherwise, it returns either a normal state, or a run time error 
+   or an abnormal state; run time checks (for example, division by 
+   zero check) are encoded inside the functional semantics;
+*)
+
+
+
+
+
+Function f_eval_stmt k (s: stack) (c: statement) {struct k}: Return stack := 
+  match k with
+  | 0 => Unterminated
+  | S k' => 
+    match c with
+    | S_Assignment ast_num x e =>
+        match f_eval_expr s e with
+        | Normal v => 
+            match updateG s x (Value v) with
+            | Some s1 => Normal s1
+            | None => Abnormal
+            end
+        | Run_Time_Error => Run_Time_Error
+        | Abnormal => Abnormal
+        | Unterminated => Unterminated
+        end
+    | S_Sequence ast_num c1 c2 =>
+        match f_eval_stmt k' s c1 with
+        | Normal s1 => f_eval_stmt k' s1 c2
+        | Run_Time_Error => Run_Time_Error
+        | Unterminated => Unterminated
+        | Abnormal => Abnormal
+        end
+    | S_If ast_num b c =>
+        match f_eval_expr s b with
+        | Normal (Bool true) => f_eval_stmt k' s c
+        | Normal (Bool false) => Normal s
+        | Run_Time_Error => Run_Time_Error
+        | Unterminated => Unterminated
+        | _ => Abnormal
+        end
+    | S_While_Loop ast_num b c => 
+        match f_eval_expr s b with
+        | Normal (Bool true) => 
+            match f_eval_stmt k' s c with
+            | Normal s1 => f_eval_stmt k' s1 (S_While_Loop ast_num b c)
+            | Run_Time_Error => Run_Time_Error
+            | Unterminated => Unterminated
+            | Abnormal => Abnormal
+            end
+        | Normal (Bool false) => Normal s
+        | Run_Time_Error => Run_Time_Error
+        | Unterminated => Unterminated
+        | _ => Abnormal
+        end
+    | S_ProcCall ast_num pbname lexp =>
+      match fetchG pbname s with
+        | Some (Procedure pb) => 
+          match copy_in s (procedure_parameter_profile pb) lexp with
+            | Normal prefx => 
+              match cut_until s pbname with
+                | Some (s_forget, s_called) =>
+                  match f_eval_decl s_called prefx (procedure_declarative_part pb) with
+                    | Normal s2 =>
+                      match f_eval_stmt k' (s2::s_called) (procedure_statements pb) with
+                        | Normal (frame::s') =>
+                          match split1 _ (List.length frame - List.length prefx) frame with
+                            | Some (slocal,prefx') =>
+                              (copy_out prefx' (procedure_parameter_profile pb) lexp (s_forget++s'))
+                            | None => Abnormal (* erronous store size *)
+                          end
+                        | Run_Time_Error => Run_Time_Error
+                        | _ => Abnormal (* erronous stack size or abnormal result *)
+                      end
+                    | Run_Time_Error => Run_Time_Error
+                    | _ => Abnormal
+                  end
+                | None => Abnormal (* procedure doesn't exist *)
+              end
+            (* left and right are not of the same type (return_state
+               store) and (return_state stack) *)
+            | Run_Time_Error => Run_Time_Error
+            | Abnormal => Abnormal
+            | Unterminated => Unterminated
+          end
+        | _ => (* None or non-procedure *) Abnormal
+      end
+    end
+  end.
+
+(* My renaming heuristic. Not perfect. *)
+Ltac semantic_rename_hyp th :=
+  match th with
+    | (do_check _ _ _ _) => fresh "hdo_check"
+    | (eval_expr _ _ Run_Time_Error) => fresh "heval_expr_rte"
+    | (eval_expr _ _ _) => fresh "heval_expr"
+    | (eval_decl _ _ _ _) => fresh "heval_decl"
+    | (eval_stmt _ _ _) => fresh "heval_stmt"
+    | (eval_bin_expr _ _ _ _) => fresh "heval_bin_expr"
+    | (eval_unary_expr _ _ _) => fresh "heval_unary_expr"
+    | (eval_literal _ = _) => fresh "heqeval_literal"
+    | (updateG _ _ _ = _) => fresh "hupdateG"
+    | (update _ _ _ = _) => fresh "hupdate"
+    | (fetchG _ _ = _) => fresh "heqfetchG"
+    | (fetch _ _ = _) => fresh "heqfetch"
+    | (Copy_in _ _ _ _) => fresh "hCopy_in"
+    | (Cut_until _ _ _ _) => fresh "hCut_until"
+    | (f_eval_expr _ _ = Run_Time_Error) => fresh "heqeval_expr_rte"
+    | (f_eval_expr _ _ = _) => fresh "heqeval_expr"
+    | (f_eval_decl _ _ _ = _) => fresh "heqeval_decl"
+    | (f_eval_stmt _ _ _ = _ ) => fresh "heqeval_stmt"
+    | (f_eval_bin_expr _ _ _ = _) => fresh "heqeval_bin_expr"
+    | (f_do_check _ _ _ = _) => fresh "heqdo_check"
+    | (stack_eq_length _ _) => fresh "hstack_eq_length"
+    | _ => default_rename_hyp th
+  end.
+Ltac rename_hyp ::= semantic_rename_hyp.
+
+Lemma eval_expr_unique: forall s e v1 v2,
+    eval_expr s e v1 ->
+    eval_expr s e v2 ->
+    v1 = v2.
+Proof.
+  intros s e v1 v2 hv1.
+  revert v2.
+  !induction hv1;!intros.
+  - subst.
+    !inversion heval_expr.
+    reflexivity.
+  - !inversion heval_expr; !intros.
+    Rinversion fetchG.    
+  - !inversion heval_expr;auto;!intros.
+    apply IHhv1 in heval_expr1.
+    discriminate.
+  - !inversion heval_expr0; !intros ; auto.
+    apply IHhv1_2 in heval_expr1.
+    discriminate.
+  - !inversion heval_expr1;auto;!intros.
+    apply f_do_check_complete in hdo_check.
+    apply f_do_check_complete in hdo_check0.
+    apply IHhv1_2 in heval_expr2.
+    apply IHhv1_1 in heval_expr3.
+    injection heval_expr2.
+    injection heval_expr3.
+    intros; subst.
+    rewrite hdo_check in hdo_check0.
+    discriminate.
+  - !inversion heval_expr1;!intros.
+    + apply IHhv1_1 in heval_expr_rte.
+      discriminate.
+    + apply IHhv1_2 in heval_expr_rte.
+      discriminate.
+    + apply f_do_check_complete in hdo_check0.
+      apply f_do_check_complete in hdo_check.
+      apply IHhv1_1 in heval_expr3.
+      apply IHhv1_2 in heval_expr2.
+      injection heval_expr3.
+      injection heval_expr2.
+      intros ; subst.
+      rewrite hdo_check in hdo_check0.
+      discriminate.
+    + apply IHhv1_1 in heval_expr3.
+      apply IHhv1_2 in heval_expr2.
+      injection heval_expr3.
+      injection heval_expr2.
+      intros ;subst.
+      rewrite (eval_bin_unique _ _ _ _ _ heval_bin_expr heval_bin_expr0) .
+      reflexivity.
+  - !inversion heval_expr;auto;!intros.
+    apply IHhv1 in heval_expr0.
+    discriminate.
+  - !inversion heval_expr;!intros.
+    + apply IHhv1 in heval_expr_rte.
+      discriminate.
+    + apply IHhv1 in heval_expr0.
+      injection heval_expr0.
+      intros ;subst.
+      rewrite (eval_unary_unique _ _ _ _ heval_unary_expr0 heval_unary_expr) .
+      reflexivity.
+Qed.    
+
+
+(** 
+    for any expression e evaluated under the state s, if it can be 
+    evaluated to a value v with respect to the relational semantics 
+    eval_expr, then the result value v should be either a normal 
+    value or a run time error;
+*)
+Lemma eval_expr_state : forall s e v,
+        eval_expr s e v -> (* v should be either a normal value or a run time error *)
+            (exists v0, v = Normal v0) \/ v = Run_Time_Error.
+Proof.
+    intros s e v h.
+    induction h;
+    try match goal with
+    | [ |- (exists v, Normal ?v1 = Normal v) \/ _ ]
+      => left; exists v1; reflexivity
+    | [ |- context [ _ \/ ?A = ?A ] ] => right; reflexivity
+    end; auto.
+Qed.
+
+(** 
+    for any statement c starting from the initial state s, if it 
+    terminates in a state s' with respect to the relational semantics 
+    eval_stmt, then the result state s' should be either a normal 
+    state or a run time error. In relational semantics eval_stmt, 
+    all statements that can go abnormal are excluded;
+*)
+Lemma eval_stmt_state : forall s c s',
+        eval_stmt s c s' -> (* s' is either a normal state or a run time error *)
+            (exists v, s' = Normal v) \/ s' = Run_Time_Error.
+Proof.
+    intros s c s' h.
+    induction h;
+    try match goal with
+    | [ |- (exists v, Normal ?v1 = Normal v) \/ _ ] => left; exists v1; reflexivity
+    | [ |- context [ _ \/ ?A = ?A ] ] => right; reflexivity
+    end; auto.
+Qed.
+
+(** * Bisimulation Between Relational And Functional Semantics *)
+
+(** bisimulation proof between f_eval_binexpr and eval_binexpr:
+    - f_eval_bin_expr_correct
+    - f_eval_bin_expr_complete
+*)
+Lemma f_eval_bin_expr_correct: forall op v1 v2 v,
+    f_eval_bin_expr op v1 v2 = Normal v ->
+    eval_bin_expr op v1 v2 v.
+Proof.
+    intros op v1 v2 v h1.
+    destruct op;
+    match goal with 
+    |[|- eval_bin_expr Divide _ _ _] => idtac
+    |[|- eval_bin_expr ?op _ _ _] =>
+        destruct v1, v2;
+        simpl in h1; inversion h1; subst;
+        constructor; auto
+    end.
+    destruct v1, v2; simpl in h1; inversion h1.
+    constructor.
+    remember (Zeq_bool n0 0) as x.
+    reflexivity.
+Qed.
+
+Lemma f_eval_bin_expr_complete: forall op v1 v2 v,
+    eval_bin_expr op v1 v2 v ->
+    f_eval_bin_expr op v1 v2 = Normal v.
+Proof.
+    intros op v1 v2 v h1.
+    induction h1;
+    rewrite <- H;
+    simpl; auto.
+Qed.
+
+(** bisimulation proof between f_eval_unaryexpr and eval_unaryexpr: 
+    - f_eval_unary_expr_correct
+    - f_eval_unary_expr_complete
+*)
+Lemma f_eval_unary_expr_correct: forall op v v',
+    f_eval_unary_expr op v = Normal v' ->
+    eval_unary_expr op v v'.
+Proof.
+  intros op v v' heq.
+  !destruct op ; simpl in heq.
+  - destruct v; inversion heq; subst.
+    constructor; auto.
+  - destruct v;destruct v';simpl in *;try discriminate.
+    injection heq.
+    intro.
+    subst.
+    constructor 2.      
+Qed.
+
+Lemma f_eval_unary_expr_complete: forall op v v',
+    eval_unary_expr op v v' ->
+    f_eval_unary_expr op v = Normal v'.
+Proof.
+  intros op v v' h1.
+  induction h1;simpl;subst;auto.
+Qed.
+
+(** ** Bisimulation between f_eval_expr and eval_expr for expression Semantics *)
+(** a help lemma to prove the theorem: f_eval_expr_correct *)
+Lemma f_eval_expr_correct1 : forall s e v,
+                        f_eval_expr s e = Normal v ->
+                            eval_expr s e (Normal v).
+Proof.
+  intros s e.
+  !!(functional induction (f_eval_expr s e); intros v0 h1; try inverts h1 as; subst).
+  - constructor;
+    reflexivity.
+  - constructor;
+    assumption.
+  - specialize (IHr _ heqeval_expr0).
+    specialize (IHr0 _ heqeval_expr).
+    introv h.
+    rewrite h.
+    econstructor.
+    + exact IHr.
+    + exact IHr0.
+    + apply f_do_check_correct.
+      auto.
+    + apply f_eval_bin_expr_correct; 
+      auto.
+  - specialize (IHr _ heqeval_expr).
+    introv h.
+    rewrite h.
+    econstructor. 
+    + exact IHr.
+    + destruct op. 
+      * simpl in h. 
+        destruct v; inversion h; subst.
+        constructor; auto.
+      * simpl in h. 
+        destruct v; inversion h; subst.
+        constructor; auto.
+Qed.
+
+
+(** another help lemma to prove the theorem: f_eval_expr_correct *)
+Lemma f_eval_expr_correct2 : forall s e,
+                        f_eval_expr s e = Run_Time_Error ->
+                            eval_expr s e Run_Time_Error.
+Proof.
+    intros s e.
+    (!! functional induction (f_eval_expr s e)); intro h;inversion h;simpl. 
+  - destruct op, v1, v2; simpl in h; inversion h.
+  - specialize (f_eval_expr_correct1 _ _ _ heqeval_expr0); intros hz1.
+    specialize (f_eval_expr_correct1 _ _ _ heqeval_expr); intros hz2.
+    eapply eval_E_Binary_Operation3.
+    apply hz1. apply hz2.
+    apply f_do_check_correct; auto.
+  - specialize (f_eval_expr_correct1 _ _ _ heqeval_expr); intros hz1.
+    specialize (IHr0 heqeval_expr_rte).
+    eapply eval_E_Binary_Operation2 with v1; auto.
+  - specialize (IHr heqeval_expr_rte).
+    constructor; assumption.
+  - destruct op;
+    destruct v; inversion h. 
+  - specialize (IHr heqeval_expr_rte).
+    constructor; assumption.
+Qed.
+
+(** *** f_eval_expr_correct *)
+(** 
+    for an expression e evaluated under the state s with respect to
+    the functional semantics f_eval_expr, whenever it returns a 
+    normal value v or terminates in a run time error, 
+    the relation between s, e and evaluation result should also be 
+    satisfied with respect to the relational semantics 'eval_expr';
+*)
+Theorem f_eval_expr_correct : forall s e v,
+                        (f_eval_expr s e = Normal v ->
+                            eval_expr s e (Normal v)) /\
+                        (f_eval_expr s e = Run_Time_Error ->
+                            eval_expr s e Run_Time_Error).
+Proof.
+    split.
+  - apply f_eval_expr_correct1.
+  - apply f_eval_expr_correct2.
+Qed.
+
+
+(** *** f_eval_expr_complete *)
+(** 
+   for any expression e, if it can be evaluated to a value v under
+   state s with respect to the relational semantics 'eval_expr', 
+   then when we evalute e under the same state s in functional
+   semantics 'f_eval_expr', it should return the same result v;
+*)
+Theorem f_eval_expr_complete : forall e s v,  
+                        eval_expr e s v -> 
+                            (f_eval_expr e s) = v.
+Proof.
+    intros e s v h.
+    !induction h; simpl; !intros;
+    repeat match goal with
+    | h: fetchG _ _ = _  |- _ => progress rewrite h
+    | h: f_eval_expr _ _ = _ |- _ => progress rewrite h
+    end;auto.
+  - rewrite heqeval_literal; reflexivity.
+  - specialize (f_do_check_complete _ _ _ _ hdo_check); intros hz1.
+    rewrite hz1.
+    reflexivity.
+  - !destruct v1; !destruct v2;
+    !destruct op;
+    !inversion heval_bin_expr; subst; simpl; auto.
+    + (* overflow check for Plus *)
+      !inversion hdo_check; !intros; subst.
+      * rewrite heq; auto.
+      * rm_false_hyp.
+    + (* overflow check for Minus *)
+      !inversion hdo_check;!intros; subst.
+      * rewrite heq; auto.
+      * rm_false_hyp.
+    + (* overflow check for Multiply *)
+      !inversion hdo_check;!intros; subst.
+      * inversion heq; subst.
+        rewrite H0; auto.
+      * rm_false_hyp.
+    + (* both division by zero check and overflow check *)
+      !inversion hdo_check;!intros; subst.
+      * inversion heq; subst.
+        rewrite H0; auto.
+      * rm_false_hyp.
+  - destruct op.
+    + !inversion heval_unary_expr.
+      auto.
+    + !inversion heval_unary_expr.
+      auto.
+Qed.
+
+
+
+
+
+
+Ltac apply_inv :=
+  try discriminate; try Rdiscriminate;
+  match goal with
+    | H:Normal _ = Normal _ |- _ => inversion H;clear H;subst 
+    | H:update _ _ (Value _) = _ |- _ => rewrite H
+    | H:updateG _ _ (Value _) = _ |- _ => rewrite H
+    | H:f_eval_stmt _ _ _ = _ |- _ => rewrite H
+    | H:f_eval_expr _ _ = _ |- _ => rewrite H
+    | H:f_eval_decl _ _ _ = _ |- _ => rewrite H
+    | H:copy_out _ _ _ _ = _ |- _ => rewrite H
+    | H:copy_in _ _ _ = _ |- _ => rewrite H
+    | H:fetch _ _ = _ |- _ => rewrite H
+    | H:fetchG _ _ = _ |- _ => rewrite H
+    | H:split2 _ _ _ = _ |- _ => rewrite H
+    | H:split1 _ _ _ = _ |- _ => rewrite H
+    | H:cut_until _ _ = _ |- _ => rewrite H
+  end;subst;simpl;auto.
+
+Ltac invle := match goal with
+    | H: (S _ <= _)%nat |- _ => (inversion H; clear H; subst; simpl)
+  end.
+
+(** a help lemma to prove the theorem: 'f_eval_stmt_complete',
+    it means that: for any statement c, starting from initial state s, 
+    if it terminates in a normal state s' within k execution steps, 
+    then for any k' greater and equal than k, it should also terminate 
+    in the same state s';
+*)
+Lemma f_eval_stmt_fixpoint: forall k s c s', 
+        f_eval_stmt k s c = Normal s' ->
+        forall k':nat, (k <= k')%nat -> 
+            f_eval_stmt k' s c = Normal s'.
+Proof.
+    intros k s c.
+    rename_after (fun _ => functional induction (f_eval_stmt k s c); simpl; intros; subst; simpl; auto;
+    repeat progress apply_inv) c.
+  - invle; repeat apply_inv.
+  - invle.
+    + repeat apply_inv.
+    + rewrite (IHr _ heqeval_stmt0);auto with arith.
+  - invle; repeat apply_inv. rewrite (IHr _ heqeval_stmt);auto with arith.
+  - invle; repeat apply_inv.
+  - invle; repeat apply_inv. rewrite (IHr _ heqeval_stmt0); auto with arith.
+  - invle; repeat apply_inv.
+  - invle; repeat apply_inv.
+    rewrite (IHr _ heqeval_stmt).
+    repeat apply_inv.
+    auto with arith.
+Qed.
+
+(** another help lemma to prove the theorem: 'f_eval_stmt_complete' *)
+Lemma f_eval_stmt_fixpoint_E: forall k s p, 
+        f_eval_stmt k s p = Run_Time_Error ->
+        forall k':nat, (k <= k')%nat -> 
+            f_eval_stmt k' s p = Run_Time_Error.
+Proof.
+    intros k s p.
+    rename_after (fun _ => functional induction (f_eval_stmt k s p)
+                  ; simpl; intros; subst; simpl; auto;
+                  repeat progress apply_inv) p.
+  - invle;
+    apply_inv.
+  - invle;
+    repeat apply_inv.
+    rewrite (f_eval_stmt_fixpoint _ _ _ _ heqeval_stmt0); auto with arith.
+  - invle;
+    repeat apply_inv.
+    specialize (IHr heqeval_stmt). 
+    rewrite IHr; auto with arith. 
+  - invle; 
+    repeat apply_inv.
+    rewrite IHr; auto with arith.
+  - invle;
+    repeat apply_inv.
+  - invle; 
+    repeat apply_inv. 
+    rewrite (f_eval_stmt_fixpoint _ _ _ _ heqeval_stmt0); auto with arith.
+  - invle; 
+    repeat apply_inv.
+    rewrite (IHr heqeval_stmt); auto with arith.    
+  - invle; 
+    repeat apply_inv.   
+  - invle; repeat apply_inv.
+    rewrite (f_eval_stmt_fixpoint _ _ _ _ heqeval_stmt); auto with arith.
+    rewrite heq0.
+    assumption.
+  - invle; repeat apply_inv.
+    rewrite  (IHr heqeval_stmt m);auto with arith.
+  - invle; repeat apply_inv.
+  - invle; repeat apply_inv.
+Qed.
+
+
+
+Ltac rm_eval_expr :=
+  match goal with 
+    | [ h: eval_expr ?s ?b ?X, h': f_eval_expr ?s ?b = ?X |- _ ] => clear h
+    | [ h: eval_expr ?s ?b ?X, h': ?X = f_eval_expr ?s ?b |- _ ] => clear h; symmetry in h'
+    | [ h: eval_expr ?s ?b ?X |- _ ] => apply f_eval_expr_complete in h
+  end; auto.
+
+
+Lemma copy_in_correct:
+  forall s prm lexp prefx,
+    copy_in s prm lexp = (Normal prefx) <->  Copy_in s prm lexp (Normal prefx).
+Proof.
+  intros s prm lexp.
+  rename_after
+    (fun _ =>
+       functional induction copy_in s prm lexp;intros;split;simpl in *;intro heq
+     ; try (inversion heq;subst;clear heq)
+     ; repeat rm_eval_expr
+     ; try repeat progress match goal with (* Rewrite induction hyp if you can *)
+                             | H: (forall _, ?X = _ <-> _)  |- _ =>
+                               rewrite <- H in *
+                           end
+     ; try (now repeat progress
+                first [ Rdiscriminate
+                      | Rinversion copy_in;auto
+                      | Rinversion f_eval_expr;auto ])) lexp.
+  - inversion_is_var heq0.
+    econstructor 2.
+    + apply IHr;auto.
+    + assumption.
+
+  - apply Copy_in_cons_in.
+    + apply IHr.
+      assumption.
+    + assumption.
+    + apply f_eval_expr_correct1.
+      assumption.
+  - constructor 1.
+Qed.
+
+
+
+Lemma copy_in_correct2:
+  forall s prm lexp,
+    copy_in s prm lexp = Run_Time_Error <->  Copy_in s prm lexp Run_Time_Error.
+Proof.
+  intros s prm lexp.
+  rename_after
+    (fun _ => functional induction copy_in s prm lexp;intros;split;simpl in *;intro heq
+     ; try (inversion heq;subst;clear heq)
+     ; repeat try rm_eval_expr
+     ; try repeat progress (* Rewrite with induction hyp as much as we can *)
+           match goal with
+             | H: (?X = _ <-> _)  |- _ =>
+               rewrite <- H in *
+           end
+     ; try (now repeat progress
+                first [ Rdiscriminate
+                      | Rinversion copy_in;auto
+                      | Rinversion f_eval_expr;auto ])) lexp.
+  - inversion_is_var heq0.
+    rewrite heq.
+    econstructor;auto.
+    rewrite <- IHr.
+    assumption.
+  - rewrite heq.
+    apply Copy_in_cons_in_rte2 with (v:=v');auto.
+    + rewrite <- IHr.
+      assumption.
+    + apply f_eval_expr_correct1.
+      assumption.
+  - apply Copy_in_cons_in_rte1;auto.
+    apply f_eval_expr_correct2.
+    assumption.
+Qed.
+
+Lemma Copy_out_stack_eq_length :
+  forall prefx prm lexp s s',
+    Copy_out prefx prm lexp s s'
+    -> stack_eq_length s s'.
+Proof.
+  intros prefx prm lexp s s' H.
+  induction H;auto.
+  - apply stack_eq_length_refl.
+    reflexivity.
+  - transitivity  σ'.
+    + eapply updateG_stack_eq_length;eauto.
+    + assumption.
+Qed.
+
+Lemma Copy_out_length :
+  forall prefx prm lexp s s',
+    Copy_out prefx prm lexp s s'
+    -> List.length s = List.length s'.
+Proof.
+  intros prefx prm lexp s s' H.
+  induction H;auto.
+  transitivity (List.length σ');auto.
+  eapply updateG_length;eauto.
+Qed.
+
+
+
+Lemma copy_out_no_rte:
+  forall prefx lprm lexp s,
+    ~ copy_out prefx lprm lexp s = Run_Time_Error.
+Proof.
+  intros prefx lprm lexp s.
+  functional induction copy_out prefx lprm lexp s;try assumption;try discriminate.
+Qed.
+
+
+Lemma copy_out_correct:
+  forall prefx s (prm:list parameter_specification) lexp x,
+    copy_out prefx prm lexp s = Normal x <-> Copy_out prefx prm lexp s x.
+Proof.
+  intros prefx s prm lexp.
+  rename_after
+    (fun _ =>
+       functional induction copy_out prefx prm lexp s;intros;split;simpl in *;intro heq
+     ; try (now (inversion heq;subst;clear heq);auto;try now (econstructor;eauto))) lexp.
+  - apply Copy_out_cons_out with (σ':=s') (v:=v)(id:=parameter_name prm);auto.
+    apply IHr.
+    assumption.
+  - !inversion heq;!intros.
+    + Rinversion fetch.
+      Rinversion updateG. 
+      apply IHr;assumption.
+    + Rdiscriminate.
+  - !inversion heq;!intros.
+    + Rinversion fetch.
+      Rdiscriminate.
+    + Rdiscriminate.
+  - !inversion heq; !intros.
+    + Rdiscriminate.
+    + Rdiscriminate.
+  - !inversion heq; !intros.
+    + contradiction.
+    + Rdiscriminate.
+  - constructor 3;auto.
+    apply IHr.
+    assumption.
+  - !inversion heq;!intros.
+    + Rdiscriminate.
+    + apply IHr.
+      assumption.
+  - !inversion heq;!intros.
+    + rewrite heq0 in y.
+      contradiction.
+    + rewrite heq0 in y.
+      contradiction.
+Qed.
+
+
+
+
+
+Lemma eval_decl_store_length:
+  forall s sto s' decl,
+    eval_decl s sto decl s'
+    -> forall st, s' = Normal st
+                  -> exists prfx, st = prfx ++ sto.
+Proof.
+  intros s sto s' decl h.
+  !induction h;intros st heq';!inversion heq';subst.
+  - exists ((object_name d, Value v)::nil).
+    simpl.
+    reflexivity.
+  - exists ((object_name d, Undefined)::nil);simpl.
+    reflexivity.
+  - destruct (IHh2 st).
+    { reflexivity. }
+    destruct (IHh1 s').
+    { reflexivity. }
+    subst.
+    exists (x ++ x0).
+    apply app_assoc.
+  - exists ((procedure_name pbody, Procedure pbody)::nil);simpl.
+    reflexivity.
+Qed.
+
+
+Lemma eval_stmt_store_length:
+  forall s s' stm,    
+    eval_stmt s stm s'
+    -> forall st, s' = Normal st
+                  -> stack_eq_length s st.
+Proof.
+  intros s s' stm H.
+  (*    !! (induction H;intros st heq';inversion heq';clear heq'; subst;auto). *)
+  (!!induction H; intros st heq'; inversion heq';clear heq'; subst;auto).
+  - apply updateG_stack_eq_length in hupdateG.
+    assumption.
+  - apply stack_eq_length_trans with s1.
+    + apply IHeval_stmt1.
+      reflexivity.
+    + apply IHeval_stmt2.
+      reflexivity.
+  - apply stack_eq_length_refl.
+    reflexivity.
+  - apply stack_eq_length_trans with s1.
+    + apply IHeval_stmt1.
+      reflexivity.
+    + apply IHeval_stmt2.
+      reflexivity.
+  - apply stack_eq_length_refl.
+    reflexivity.
+  - generalize (Cut_until_def _ _ _ _ hCut_until).
+    intros hcutin.
+    subst.
+    specialize (IHeval_stmt ((slocal ++ prefix') :: s') eq_refl).
+    !inversion IHeval_stmt;!intros.
+    rewrite hstack_eq_length.
+    eapply Copy_out_stack_eq_length;eauto.
+Qed.
+
+Lemma f_eval_decl_correct :
+  forall s sto d s',
+    f_eval_decl s sto d = Normal s' ->
+    eval_decl s sto d (Normal s').
+Proof.
+  intros s sto d.
+  functional induction f_eval_decl s sto d;simpl;intros;try discriminate
+  ; try match goal with
+        | H: Normal _ = Normal _ |- _ =>
+          inversion H;subst;clear H
+      end;try now( (econstructor;eauto;try apply f_eval_expr_correct1;auto)).
+  - rewrite H in y.
+    contradiction.
+Qed.
+
+Lemma f_eval_decl_correct2 :
+  forall s sto d,
+    f_eval_decl s sto d = Run_Time_Error ->
+    eval_decl s sto d Run_Time_Error.
+Proof.
+  intros s sto d.
+  functional induction f_eval_decl s sto d;simpl;intros;try discriminate;
+  try match goal with
+        | H: Normal _ = Run_Time_Error |- _ =>
+          inversion H;subst;clear H
+      end;try now( (econstructor;eauto);try apply f_eval_expr_correct2;auto).
+  
+  eapply eval_decl_Seq_err2 with s';auto.
+  apply f_eval_decl_correct.
+  assumption.
+Qed.
+
+Ltac use_determinism :=
+  match goal with
+    | H : ?X = ?X |- _ => clear H
+    | H: None = ?y, H': ?y = Some ?z |- _ => rewrite H' in H; !invclear H
+    | H: Some ?z = ?y, H': ?y = None |- _ => rewrite H' in H; !invclear H
+    | H: Some ?x = ?y, H': ?y = Some ?z |- _ => rewrite H' in H; !invclear H
+    | H : eval_expr ?s ?e ?X,
+          H': f_eval_expr ?s ?e = ?Y |- _ => rewrite (f_eval_expr_complete s e X H) in H'
+    | H:  eval_expr ?s ?e ?X,
+          H': eval_expr ?s ?e ?Y |- _ => apply (f_eval_expr_complete s e X) in H
+         ;apply (f_eval_expr_complete s e) in H'
+    | H : f_eval_expr ?s ?e = ?X,
+          H': f_eval_expr ?s ?e = ?Y |- _ => rewrite H in H'; !invclear H'
+    | H : (Normal ?v) = (Normal ?v') |- _ => !invclear H
+  end.
+
+Ltac crush := repeat progress use_determinism;try reflexivity;try discriminate.
+
+
+Lemma f_eval_decl_complete :
+  forall d sto s s',
+    eval_decl s sto d s' ->
+    f_eval_decl s sto d = s'.
+Proof.
+  intros d sto s.
+  (!!functional induction f_eval_decl s sto d);simpl;!intros;try discriminate;crush;
+  try now (!inversion heval_decl;!intros;crush).
+  - !inversion heval_decl;!intros.
+    + apply IHr in heval_decl1.
+      Rinversion f_eval_decl.
+    + apply IHr in heval_decl0.
+      Rinversion f_eval_decl.
+    + apply IHr in heval_decl1.
+      Rinversion f_eval_decl.
+  - !inversion heval_decl;!intros.
+    + apply IHr in heval_decl1.
+      Rinversion f_eval_decl.
+    + apply IHr in heval_decl0.
+      assumption.
+    + apply IHr in heval_decl1.
+      rewrite heval_decl1 in y.
+      contradiction.
+Qed.
+
+
+(** ** Bisimulation between f_eval_stmt and eval_stmt for statement semantics *)
+
+
+Ltac rm_f_eval_expr :=
+  match goal with 
+    | [ h: f_eval_expr ?s ?b = Run_Time_Error |- _ ] => 
+      specialize (f_eval_expr_correct2 _ _ h);
+        !intros
+    | [ h: f_eval_expr ?s ?b = Normal ?v |- _ ] => 
+      specialize (f_eval_expr_correct1 _ _ _ h);
+        !intros
+  end; auto.
+
+
+
+(** a help lemma to prove the theorem: 'f_eval_stmt_complete' *)
+Lemma f_eval_stmt_correct1 : forall k s p s',
+        f_eval_stmt k s p = Normal s' ->
+          eval_stmt s p (Normal s').
+Proof.
+    intros k s p.
+    !!(functional induction (f_eval_stmt k s p);
+       intros; try inversion H; subst).
+  - (* S_Assignment *)
+    econstructor.
+    rm_f_eval_expr.
+    apply heval_expr.
+    assumption.
+  - (* S_Sequence *)
+    specialize (IHr _ heqeval_stmt1).
+    specialize (IHr0 _ heqeval_stmt).
+    econstructor.
+    apply IHr.
+    apply_inv.
+  - (* S_If_True *)
+    specialize (IHr _ heqeval_stmt).
+    econstructor.
+    rm_f_eval_expr. 
+    apply_inv.
+  - (* S_If_False *)
+    eapply eval_S_If_False.
+    rm_f_eval_expr.
+  - (* S_While_Loop_True *)
+    specialize (IHr _ heqeval_stmt1).
+    specialize (IHr0 _ heqeval_stmt).
+    econstructor.
+    rm_f_eval_expr.
+    apply IHr. 
+    apply_inv.
+  - (* S_While_Loop_False *)
+    eapply eval_S_While_Loop_False.
+    rm_f_eval_expr.
+  - (* S_ProcCall *)
+    clear heq0.
+    (* cleaning by going to inductive defs *)
+    apply split1_correct in heq1.
+    destruct heq1 as [hsplit1 hsplit2].
+    rewrite heq.
+    subst.
+    apply f_eval_decl_correct in heqeval_decl.    
+    apply IHr in heqeval_stmt.
+    apply copy_in_correct in heq3.
+    apply copy_out_correct in heq.
+    (* ******* *)
+    eapply eval_S_Proc with (s':=s') (prefix':=prefx')(prefix:=prefx)(slocal:=slocal);eauto.
+    + apply cut_until_complete1.
+      assumption.
+    + eapply eval_decl_store_length with (st:=s2) in heqeval_decl;auto.
+      destruct heqeval_decl as [slocal' ?].
+      subst.
+      apply eval_stmt_store_length with (st:=((slocal ++ prefx') :: s')) in heqeval_stmt;auto.
+      !invclear heqeval_stmt.
+      rewrite <- heq0 in hsplit1.
+      setoid_rewrite app_length in heq0.
+      setoid_rewrite app_length in hsplit1.
+      omega.
+Qed.
+
+
+Ltac rm_f_eval_stmt :=
+    match goal with 
+    | [ h: f_eval_stmt ?k ?s ?c = Normal ?s1 |- _ ] => 
+        specialize (f_eval_stmt_correct1 _ _ _ _ h);
+        !intros
+    end; auto.
+
+(** a help lemma to prove the theorem: 'f_eval_stmt_complete' *)
+Lemma f_eval_stmt_correct2 : forall k s p,
+        f_eval_stmt k s p = Run_Time_Error ->
+          eval_stmt s p Run_Time_Error.
+Proof.
+    intros k s p.
+    !!(functional induction (f_eval_stmt k s p);intros;try discriminate).
+(*     !!(functional induction (f_eval_stmt k s p)); intros H ; try inversion H; subst. *)
+  - (* S_Assignment *)
+    econstructor.
+    rm_f_eval_expr.
+  - (* S_Sequence*)
+    eapply eval_S_Sequence2.
+    + rm_f_eval_stmt.
+      eauto.
+    + apply IHr0.
+      assumption.
+  - specialize (IHr heqeval_stmt).
+    econstructor.
+    assumption.    
+  - (* C_If *)
+    specialize (IHr heqeval_stmt).
+    eapply eval_S_If_True.
+    rm_f_eval_expr.
+    assumption.
+  - eapply eval_S_If .
+    rm_f_eval_expr.
+  (* S_While_Loop *)
+  - eapply eval_S_While_Loop_True2.
+    + apply f_eval_expr_correct1.
+      assumption.
+    + rm_f_eval_stmt.
+      eauto.
+    + apply IHr0.
+      assumption.
+  - eapply eval_S_While_Loop_True1;auto.
+    rm_f_eval_expr.
+
+  - (* S_While_Loop *)
+    apply eval_S_While_Loop.
+    rm_f_eval_expr.
+  - elim (copy_out_no_rte _ _ _ _ heq).
+  - apply eval_S_Proc_rtebody with 
+    (prefix:=prefx)
+      (s2:=s2)
+      (s:=s_called)
+      (s_forget:=s_forget)
+      (pb:=pb);auto. 
+    + apply copy_in_correct.
+      assumption.
+    + apply cut_until_complete1.
+      assumption.
+    + apply f_eval_decl_correct.
+      assumption.
+  - apply eval_S_Proc_rtedecl
+    with (prefix:=prefx) (pb:=pb) (s_forget:=s_forget) (s:=s_called)
+    ;eauto.
+    + apply copy_in_correct.
+      assumption.
+    + apply cut_until_complete1.
+      assumption.
+    + eapply f_eval_decl_correct2.
+      assumption.
+  - eapply eval_S_Proc_rteargs with pb;auto.
+    apply copy_in_correct2.
+    assumption.
+Qed.
+    
+    
+
+Ltac rm_f_eval :=
+    match goal with 
+    | [ h: f_eval_expr ?s ?b = Run_Time_Error |- _ ] => specialize (f_eval_expr_correct2 _ _ h); intros hz1
+    | [ h: f_eval_expr ?s ?b = Normal ?v |- _ ] => specialize (f_eval_expr_correct1 _ _ _ h); intros hz1   
+    | [ h: f_eval_stmt ?k ?s ?c = Run_Time_Error |- _ ] => specialize (f_eval_stmt_correct2 _ _ _ h); intros hz1
+    | [ h: f_eval_stmt ?k ?s ?c = Normal ?s1 |- _ ] => specialize (f_eval_stmt_correct1 _ _ _ _ h); intros hz1
+    end; auto.
+
+(** *** f_eval_stmt_correct *)
+(** 
+   for any statement c starting from initial state s, if it returns 
+   a normal state s' or terminates in a run time error within k steps
+   with respect to the functional semantics 'f_eval_stmt', then the 
+   relation between s, c and the resulting state should also be 
+   satisfied with respect to the relational semantics 'eval_stmt';
+*)
+Theorem f_eval_stmt_correct : forall k s c s',
+        (f_eval_stmt k s c = Normal s' ->
+          eval_stmt s c (Normal s')) /\ 
+        (f_eval_stmt k s c = Run_Time_Error ->
+          eval_stmt s c Run_Time_Error).
+Proof.
+    intros.
+    split; intros;
+    rm_f_eval.
+Qed.
+
+(** *** f_eval_stmt_complete *)
+(** 
+   the reverse direction is also satisfied: for any statement c, 
+   whenever it's executed starting from initial state s and return 
+   a new state s' with regard to the relational semantics 'eval_stmt', 
+   then there should exist a constant k that statement c starting from 
+   s will terminate in state s' within k steps with respect to the 
+   functional semantics 'f_eval_stmt';
+*)
+
+Ltac apply_rewrite := 
+    match goal with
+    | h: eval_expr ?s ?e ?s' |- _ => 
+        rewrite (f_eval_expr_complete _ _ _ h)
+    | h: update _ _ _ = _ |- _ => rewrite h
+    | h: updateG _ _ _ = _ |- _ => rewrite h
+    | h: f_eval_stmt _ _ _ = _ |- _ => rewrite h
+    | h: f_eval_expr _ _ = _ |- _ => rewrite h
+    | h: fetch _ _ = _ |- _ => rewrite h
+    | h: fetchG _ _ = _ |- _ => rewrite h
+    | h: copy_in _ _ _ = _ |- _ => rewrite h
+    | h: Copy_in _ _ _ Run_Time_Error |- _ => rewrite <- copy_in_correct2 in h;rewrite h
+    | h: Copy_in _ _ _ (Normal _) |- _ => rewrite <- copy_in_correct in h;rewrite h
+    | h: cut_until _ _ = Some(_, _) |- _ => rewrite h
+    | h: cut_until _ _ = None |- _ => rewrite h
+    | h: Cut_until _ _ _ _ |- _ => apply cut_until_correct in h;rewrite h
+    end; auto.
+
+
+Ltac kgreater :=
+  repeat
+    match goal with
+      | h:f_eval_stmt ?k ?s ?p = Normal ?s' |- context [f_eval_stmt (?k + _) ?s ?p] =>
+        rewrite (@f_eval_stmt_fixpoint _ _ _ _ h);auto with arith
+      | h:f_eval_stmt ?k ?s ?p = Normal ?s' |- context [f_eval_stmt (_ + ?k) ?s ?p] =>
+        rewrite (@f_eval_stmt_fixpoint _ _ _ _ h);auto with arith
+      | h:f_eval_stmt ?k ?s ?p = Run_Time_Error |- context [f_eval_stmt (?k + _) ?s ?p] =>
+        rewrite (@f_eval_stmt_fixpoint_E _ _ _ h);auto with arith
+      | h:f_eval_stmt ?k ?s ?p = Run_Time_Error |- context [f_eval_stmt (_ + ?k) ?s ?p] =>
+        rewrite (@f_eval_stmt_fixpoint_E _ _ _ h);auto with arith
+         end.
+
+
+
+Theorem f_eval_stmt_complete : forall s c s',
+        eval_stmt s c s' -> (* s' is either a normal state or a run time error *)
+            exists k, f_eval_stmt k s c = s'.
+Proof. 
+  !intros.
+  !induction heval_stmt;
+  try match goal with
+  [ h: eval_expr ?s ?e Run_Time_Error |- exists k, _ = Run_Time_Error] => 
+          exists 1%nat; simpl;
+          rewrite (f_eval_expr_complete _ _ _ h);
+          reflexivity
+  end.
+  (* 1. S_Assignment *)
+  - exists 1%nat; simpl.
+    repeat apply_rewrite.
+  (* 2. S_Sequence *)
+  - destrEx.
+    exists (S k); simpl.
+    apply_rewrite.
+  - destrEx.
+    exists (S (k0+k)); simpl.
+    kgreater.
+    specialize (eval_stmt_state _ _ _ heval_stmt); intros hz1.
+    destruct hz1 as [hz2 | hz2]; try rm_exists; subst;
+    kgreater.
+  (* 3. S_If *)
+  - destrEx.
+    exists (S k); simpl.
+    apply_rewrite.
+  - exists 1%nat; simpl.
+    apply_rewrite.
+  (* 4. S_While_Loop *)
+  - destrEx.
+    exists (S k); simpl.
+    repeat apply_rewrite.
+  - destrEx.
+    exists (S (k0+k)); simpl.
+    apply_rewrite.
+    kgreater.
+    specialize (eval_stmt_state _ _ _ heval_stmt); intros hz1.
+    destruct hz1 as [hz2 | hz2]; try rm_exists; subst;
+    kgreater.
+  - exists 1%nat; simpl.
+    apply_rewrite.
+  - exists 1%nat; simpl.
+    repeat progress apply_rewrite.
+  - exists 1%nat; simpl.
+    subst.
+    repeat apply_rewrite.
+    apply f_eval_decl_complete in heval_decl.
+    rewrite heval_decl.
+    reflexivity.
+  - destruct IHheval_stmt as [k IH].
+    exists (S k).
+    simpl.
+    repeat apply_rewrite.
+    apply f_eval_decl_complete in heval_decl.
+    rewrite heval_decl.
+    apply_rewrite.
+  - destruct IHheval_stmt as [k IH].
+    exists (S k).
+    simpl.
+    subst.
+    repeat apply_rewrite.
+    apply f_eval_decl_complete in heval_decl.
+    rewrite heval_decl.
+    repeat apply_rewrite.
+    repeat setoid_rewrite app_length.
+    rewrite heq.
+    assert (heq':Datatypes.length slocal + Datatypes.length prefix' -
+        Datatypes.length prefix' = Datatypes.length slocal) by omega.
+    rewrite heq'.
+    rewrite split1_complete with (l2:=prefix') (l1:=slocal).
+    + apply copy_out_correct.
+      assumption.
+    + reflexivity.
+    + reflexivity.
+Qed.
+
+(**********************************************************************)
+(**********************************************************************)
+
+(** * Subprogram Semantics *)
+
+(** In the current SPARK subset, there is no procedure call, 
+    so right now we only define the semantics for the main procedure.
+    And it can be used to test the tool chain from SPARK source code 
+    to Coq evaluation; Later, we will add the procedure call and 
+    modify the following procedure semantics;
+*)
+
+(** all declared variables in the same procedure should have unique 
+    names; 
+*)
+
+(** relational (eval_decl) and functional (f_eval_decl) semantics for 
+    variable declaration;
+*)
+
+(** for any initial state s, after executing the declaration d, 
+    it either returns a normal state s' or a run time error;
+    (for any variable declaration, if its initialization expression 
+     fails the run time checks, for example division by zero or overflow, 
+     then it returns an exception)
+*)
+
+Lemma eval_decl_state : forall s sto d s',
+        eval_decl s sto d s' -> (* s' is either a normal state or a run time error *)
+            (exists t, s' = Normal t) \/ s' = Run_Time_Error.
+Proof.
+    intros s sto d s' h.
+    induction h;
+    try match goal with
+    | [ |- (exists t, Normal ?t1 = Normal t) \/ _ ] => left; exists t1; reflexivity
+    | [ |- context [ _ \/ ?A = ?A ] ] => right; reflexivity
+    end; auto.
+Qed.
+
+
+(** f_eval_decl completeness and correctness proofs *)
+
+(** bisimulation proof between f_eval_decl and eval_decl: 
+    - f_eval_decl_correct
+    - f_eval_decl_complete
+*)
+
+Lemma f_eval_decl_correct_: forall d s sto s',
+    (f_eval_decl s sto d = (Normal s') -> eval_decl s sto d (Normal s')) /\
+    (f_eval_decl s sto d = Run_Time_Error -> eval_decl s sto d Run_Time_Error).
+Proof.
+    intros d s sto.
+    intros s'.
+    split;intro h.
+    - apply f_eval_decl_correct.
+      assumption.
+    - apply f_eval_decl_correct2.
+      assumption.
+Qed.
+
+
+(* = = = = = = Subprogram Body = = = = = =  *)
+(** relational and functional semantics for procedure body; *)
+(* Is this still needed for global procedures? probably not. *)
+(* main procedure has no argument, so we give the nil store as
+   parameter store *)
+Inductive eval_proc: stack -> procedure_declaration -> Return stack -> Prop :=
+    | eval_Proc_E: forall f s,
+        eval_decl s nil (procedure_declarative_part f) Run_Time_Error ->
+        eval_proc s f Run_Time_Error
+    | eval_Proc: forall f s1 s2 s3,
+        eval_decl s1 nil (procedure_declarative_part f) (Normal s2) ->
+        eval_stmt (s2::s1) (procedure_statements f) s3 ->
+        eval_proc s1 f s3.
+
+Function f_eval_proc k (s: stack) (f: procedure_declaration): Return stack :=
+    match (f_eval_decl s nil (procedure_declarative_part f)) with
+    | Normal s' => f_eval_stmt k (s'::s) (procedure_statements f)
+    | Run_Time_Error => Run_Time_Error
+    | Abnormal => Abnormal
+    | Unterminated => Unterminated
+    end.
+
+
+(** ** Main Procedure Evaluation Without Parameters *)
+
+(** relational and functional semantics for main procedure; *)
+
+Inductive eval_subprogram: stack -> subprogram -> Return stack -> Prop :=
+    | eval_Procedure: forall s s' ast_num f,
+        eval_proc s f s' ->
+        eval_subprogram s (Global_Procedure ast_num f) s'.
+
+Function f_eval_subprogram k (s: stack) (f: subprogram): Return stack := 
+    match f with 
+    | Global_Procedure ast_num f' => f_eval_proc k s f'
+    end.
+
+(** ** Bisimulation Between Relational And Functional Semantics For Main Procedure *)
+
+(** *** f_eval_subprogram_correct *)
+Theorem f_eval_subprogram_correct: forall k s f s',
+    (f_eval_subprogram k s f = Normal s' -> 
+        eval_subprogram s f (Normal s')) /\
+    (f_eval_subprogram k s f = Run_Time_Error -> 
+        eval_subprogram s f Run_Time_Error).
+Proof.
+    intros.
+    !! (split; intros;
+        destruct f;
+        simpl in H;
+        constructor;
+        unfold f_eval_proc in H ;
+        remember (f_eval_decl s nil (procedure_declarative_part p)) as x;
+        symmetry in Heqx).
+  - (* normal state *)
+    destruct x; !invclear heq.
+    econstructor.
+    + apply f_eval_decl_correct.
+      apply heqeval_decl.
+    + rewrite heqeval_stmt.
+      apply f_eval_stmt_correct in heqeval_stmt;assumption.
+  - (* run time error *)
+    destruct x; !invclear heq; subst.
+    + econstructor.
+       * apply f_eval_decl_correct in heqeval_decl.
+         apply heqeval_decl.
+       * rewrite heqeval_stmt.
+         apply f_eval_stmt_correct in heqeval_stmt; assumption.
+    + econstructor.
+      apply f_eval_decl_correct2 in heqeval_decl; assumption.
+Qed.
+
+(** *** f_eval_subprogram_complete *)
+Theorem f_eval_subprogram_complete: forall s f s',
+    eval_subprogram s f s' ->
+    exists k, f_eval_subprogram k s f = s'.
+Proof.
+  intros s f s' h.
+  unfold f_eval_subprogram.
+  unfold f_eval_proc.
+  !invclear h.
+  !invclear H;simpl.
+  - exists 0.
+    apply f_eval_decl_complete in heval_decl.
+    rewrite heval_decl.
+    reflexivity.
+  - apply f_eval_decl_complete in heval_decl.
+    rewrite heval_decl.
+    apply f_eval_stmt_complete in heval_stmt.
+    assumption.
+Qed.
+
+(** * Replaying examples using the correctness of functional semantics *)
+Module ExampleProcedures2.
+(* EXAMPLE 1, v102 is a variable in the scope.
+------------------------
+procedure P2 () is
+  V4 : TYPE5 := 34;
+begin
+  V102 := 56;
+end 
+-----------------------
+*)
+Definition proc1:procedure_declaration := (mkprocedure_declaration
+           1 2 nil nil
+             (D_Object_declaration
+                {|
+                  declaration_astnum := 3;
+                  object_name := 4;
+                  object_nominal_subtype :=  5;
+                  initialization_expression := Some (E_Literal 6 (Integer_Literal(34)))
+                |}
+             )
+             (S_Assignment 12 102 (E_Literal 8 (Integer_Literal(56))))).
+
+Definition s1:store := (101,Procedure proc1) :: (102, Value (Int(77))) :: nil.
+
+Definition s2:store := (101,Procedure proc1) :: (102, Value (Int(56)))  :: nil.
+
+Eval vm_compute in f_eval_stmt 200 (s1::nil) (S_ProcCall 13 101 nil).
+
+Lemma essai: eval_stmt (s1::nil) (S_ProcCall 13 101 nil) (Normal (s2::nil)).
+Proof.
+  apply f_eval_stmt_correct1 with (k:=2).
+  compute.f_eval_proc k s f'
+    end.
+
+(** ** Bisimulation Between Relational And Functional Semantics For Main Procedure *)
+
+(** *** f_eval_subprogram_correct *)
+Theorem f_eval_subprogram_correct: forall k s f s',
+    (f_eval_subprogram k s f = Normal s' -> 
+        eval_subprogram s f (Normal s')) /\
+    (f_eval_subprogram k s f = Run_Time_Error -> 
+        eval_subprogram s f Run_Time_Error).
+Proof.
+    intros.
+    !! (split; intros;
+        destruct f;
+        simpl in H;
+        constructor;
+        unfold f_eval_proc in H ;
+        remember (f_eval_decl s nil (procedure_declarative_part p)) as x;
+        symmetry in Heqx).
+  - (* normal state *)
+    destruct x; !invclear heq.
+    econstructor.
+    + apply f_eval_decl_correct.
+      apply heqeval_decl.
+    + rewrite heqeval_stmt.
+      apply f_eval_stmt_correct in heqeval_stmt;assumption.
+  - (* run time error *)
+    destruct x; !invclear heq; subst.
+    + econstructor.
+       * apply f_eval_decl_correct in heqeval_decl.
+         apply heqeval_decl.
+       * rewrite heqeval_stmt.
+         apply f_eval_stmt_correct in heqeval_stmt; assumption.
+    + econstructor.
+      apply f_eval_decl_correct2 in heqeval_decl; assumption.
+Qed.
+
+(** *** f_eval_subprogram_complete *)
+Theorem f_eval_subprogram_complete: forall s f s',
+    eval_subprogram s f s' ->
+    exists k, f_eval_subprogram k s f = s'.
+Proof.
+  intros s f s' h.
+  unfold f_eval_subprogram.
+  unfold f_eval_proc.
+  !invclear h.
+  !invclear H;simpl.
+  - exists 0.
+    apply f_eval_decl_complete in heval_decl.
+    rewrite heval_decl.
+    reflexivity.
+  - apply f_eval_decl_complete in heval_decl.
+    rewrite heval_decl.
+    apply f_eval_stmt_complete in heval_stmt.
+    assumption.
+Qed.
+
+
+  reflexivity.
+Qed.
+
+
+
+(* v102 is a variable in the scope.
+procedure P2 () is
+  V4 : TYPE5 := 34;
+  V5 : TYPE5 := 37;
+begin
+  V5 := V4 + V5;
+  V102 := V5*2;
+end 
+*)
+Definition proc2:procedure_declaration := (mkprocedure_declaration
+           1 2 nil nil
+             (D_Sequence
+                (D_Object_declaration
+                   {|
+                     declaration_astnum := 3;
+                     object_name := 4;
+                     object_nominal_subtype :=  5;
+                     initialization_expression := Some (E_Literal 6 (Integer_Literal(34)))
+                   |}
+                )
+                (D_Object_declaration
+                   {|
+                     declaration_astnum := 4;
+                     object_name := 5;
+                     object_nominal_subtype :=  5;
+                     initialization_expression := Some (E_Literal 6 (Integer_Literal(37)))
+                   |}
+                )
+             )
+             (S_Sequence 13
+                (S_Assignment 14 5
+                              (E_Binary_Operation 9 Plus
+                                                  (E_Identifier 10 5)
+                                                  (E_Identifier 10 4)))
+                (S_Assignment
+                   12
+                   102
+                   (E_Binary_Operation 9 Multiply
+                                       (E_Identifier 10 5)
+                                       (E_Literal 8 (Integer_Literal(2))))))).
+
+Definition s3:store := (101,Procedure proc2) :: (102, Value (Int(77))) :: nil.
+
+Definition s4:store := (101,Procedure proc2) :: (102, Value (Int(142)))  :: nil.
+
+
+Lemma essai2: eval_stmt (s3::nil) (S_ProcCall 13 101 nil) (Normal (s4::nil)).
+Proof.
+  apply f_eval_stmt_correct1 with (k:=200).
+  vm_compute.
+  reflexivity.
+Qed.
+
+
+End ExampleProcedures2.
+(* END EXAMPLE *)
